añadi la carpeta ProyatoCoq

ProyectoCoq/.Makefile.d
@@ -1,0 +1,24 @@
+Bumcrot.vo Bumcrot.glob Bumcrot.v.beautified Bumcrot.required_vo: Bumcrot.v Def_Lattice.vo Dualidad.vo Dualidad_Bumcrot.vo MathCompLattices_SeqEnv.vo
+Bumcrot.vio: Bumcrot.v Def_Lattice.vio Dualidad.vio Dualidad_Bumcrot.vio MathCompLattices_SeqEnv.vio
+Bumcrot.vos Bumcrot.vok Bumcrot.required_vos: Bumcrot.v Def_Lattice.vos Dualidad.vos Dualidad_Bumcrot.vos MathCompLattices_SeqEnv.vos
+Curry.vo Curry.glob Curry.v.beautified Curry.required_vo: Curry.v Def_Lattice.vo Dualidad.vo Ltac_Dual.vo CurryThm2.vo
+Curry.vio: Curry.v Def_Lattice.vio Dualidad.vio Ltac_Dual.vio CurryThm2.vio
+Curry.vos Curry.vok Curry.required_vos: Curry.v Def_Lattice.vos Dualidad.vos Ltac_Dual.vos CurryThm2.vos
+CurryThm2.vo CurryThm2.glob CurryThm2.v.beautified CurryThm2.required_vo: CurryThm2.v Def_Lattice.vo
+CurryThm2.vio: CurryThm2.v Def_Lattice.vio
+CurryThm2.vos CurryThm2.vok CurryThm2.required_vos: CurryThm2.v Def_Lattice.vos
+Def_Lattice.vo Def_Lattice.glob Def_Lattice.v.beautified Def_Lattice.required_vo: Def_Lattice.v 
+Def_Lattice.vio: Def_Lattice.v 
+Def_Lattice.vos Def_Lattice.vok Def_Lattice.required_vos: Def_Lattice.v 
+Dualidad.vo Dualidad.glob Dualidad.v.beautified Dualidad.required_vo: Dualidad.v Def_Lattice.vo
+Dualidad.vio: Dualidad.v Def_Lattice.vio
+Dualidad.vos Dualidad.vok Dualidad.required_vos: Dualidad.v Def_Lattice.vos
+Dualidad_Bumcrot.vo Dualidad_Bumcrot.glob Dualidad_Bumcrot.v.beautified Dualidad_Bumcrot.required_vo: Dualidad_Bumcrot.v Def_Lattice.vo Dualidad.vo MathCompLattices_SeqEnv.vo
+Dualidad_Bumcrot.vio: Dualidad_Bumcrot.v Def_Lattice.vio Dualidad.vio MathCompLattices_SeqEnv.vio
+Dualidad_Bumcrot.vos Dualidad_Bumcrot.vok Dualidad_Bumcrot.required_vos: Dualidad_Bumcrot.v Def_Lattice.vos Dualidad.vos MathCompLattices_SeqEnv.vos
+Ltac_Dual.vo Ltac_Dual.glob Ltac_Dual.v.beautified Ltac_Dual.required_vo: Ltac_Dual.v Def_Lattice.vo Dualidad.vo
+Ltac_Dual.vio: Ltac_Dual.v Def_Lattice.vio Dualidad.vio
+Ltac_Dual.vos Ltac_Dual.vok Ltac_Dual.required_vos: Ltac_Dual.v Def_Lattice.vos Dualidad.vos
+MathCompLattices_SeqEnv.vo MathCompLattices_SeqEnv.glob MathCompLattices_SeqEnv.v.beautified MathCompLattices_SeqEnv.required_vo: MathCompLattices_SeqEnv.v Def_Lattice.vo Dualidad.vo Ltac_Dual.vo
+MathCompLattices_SeqEnv.vio: MathCompLattices_SeqEnv.v Def_Lattice.vio Dualidad.vio Ltac_Dual.vio
+MathCompLattices_SeqEnv.vos MathCompLattices_SeqEnv.vok MathCompLattices_SeqEnv.required_vos: MathCompLattices_SeqEnv.v Def_Lattice.vos Dualidad.vos Ltac_Dual.vos
