ProyectoCoq/CurryThm2.v
@@ -1,0 +1,141 @@
+From mathcomp Require Import all_ssreflect.
+From ProyectoCoq Require Import Def_Lattice.
+
+Notation ρ := (reflexT _).
+Notation τ := (transT _).
+Notation σ := (antisymT _).
+
+Lemma ΛK {T : lattice} (z : T) : forall a b : T ,  (a ⊓ b) ≤ a.
+Proof.
+move=> a b.
+move: (ρ (a ⊓ b)).
+by rewrite -(MH (a ⊓ b) a b) => /proj1.
+Qed.
+
+Lemma ΛK' {T : lattice} (z : T) : forall a b : T , (a ⊓ b) ≤ b.
+Proof.
+move=> a b.
+move: (ρ (a ⊓ b)).
+by rewrite -(MH (a ⊓ b) a b) => /proj2.
+Qed.
+
+Lemma ΛS {T : lattice} (z : T) : forall a b c : T , ((c ≤ a /\ c ≤ b) -> c ≤ (a ⊓ b)).
+Proof.
+move=> a b c.
+by move: (MH c a b) => /proj1.
+Qed.
+
+Inductive STerm : Set := 
+| svar : nat -> STerm
+| sOp  : STerm -> STerm -> STerm.
+
+Fixpoint evalS (sL : lattice) (z : sL) (env : seq sL) (t : STerm)  : sL :=
+  match t with
+  | svar n => nth z env n
+  | sOp t1 t2 => evalS sL z env t1 ⊓ evalS sL z env t2
+  end.
+
+Inductive SForm : Set :=
+| fs_leq  : STerm -> STerm -> SForm
+| fs_eq   : STerm -> STerm -> SForm.
+
+Fixpoint evalS_f (L : lattice) (z : L) (env : seq L) (f : SForm) : Prop :=
+  match f with
+  | fs_leq t1 t2 => (evalS L z env t1) ≤ (evalS L z env t2)
+  | fs_eq t1 t2  => (evalS L z env t1) = (evalS L z env t2)
+  end.
+
+Definition Leq (s t : STerm) : Prop := forall L z env, evalS L z env s  ≤ evalS L z env t.
+
+Definition Equiv (s t : STerm) : Prop := forall L z env, evalS L z env s = evalS L z env t.
+
+Fixpoint atm_en (s : STerm) (j : nat) :=
+  match s with
+  | svar i => i = j
+  | sOp s1 s2 => (atm_en s1 j) \/ (atm_en s2 j)
+  end.
+
+Fixpoint leq (s t : STerm) :=
+  match t with
+  | svar j => atm_en s j
+  | sOp t1 t2 => (leq s t1) /\ (leq s t2)
+  end.
+
+Lemma atm_en_eval_le (sL : lattice) (z : sL) (env : seq sL) (s : STerm) j :
+  atm_en s j -> evalS sL z env s ≤ nth z env j.
+Proof.
+elim s =>  [i|s1 H1 s2 H2] /=.
+  move=> H.
+  rewrite H.
+  by move: (ρ (nth z env j)).
+  move=> [H|H].
+    move: (ΛK z (evalS sL z env s1) (evalS sL z env s2 ))=> Hle.
+    apply (τ (evalS sL z env s1 ⊓ evalS sL z env s2) (evalS sL z env s1) _ ).
+      by [].
+    by move: H => /H1.
+move: (ΛK' z (evalS sL z env s1) (evalS sL z env s2))=> Hle.
+apply (τ (evalS sL z env s1 ⊓ evalS sL z env s2) (evalS sL z env s2) _ ).
+  by [].
+by move: H => /H2.
+Qed.
+
+Lemma leq_impl_Leq s t :
+  leq s t -> Leq s t.
+Proof.
+elim: t => [j|t1 H1 t2 H2] /=.
+  move=> H sL z env.
+  rewrite {2}/evalS.
+  by move: ((atm_en_eval_le sL z env s j) H).
+move=> [Hs1 Hs2] sL0 z0 env0.
+apply: (ΛS z0).
+split.
+  by apply: H1.
+by apply: H2.
+Qed.
+
+
+Ltac rankS env n v :=
+  match env with
+  | (cons ?X1 ?X2) =>
+      let env' := constr:(X2) in
+        match constr:(X1 = v) with
+        | (?X1 = ?X1) => n
+        | _ => rankS env' (S n) v
+        end
+  end.
+
+Ltac reflectS env m v :=
+  match v with
+  | (m _ ?X1 ?X2) =>
+      let r1 := reflectS env m X1
+      with r2 := reflectS env m X2 in
+        constr:(sOp r1 r2)
+  | ?X1 =>
+      let n := rankS env 0 X1 in
+        constr:(svar n)
+  | _ => constr:(svar 0)
+  end.
+
+Ltac reflect_formS env m f :=
+  lazymatch f with
+  | ?x ≤ ?y =>
+        let rx := reflectS env m x in
+        let ry := reflectS env m y in
+        constr:(fs_leq rx ry)
+  | ?x = ?y =>
+        let rx := reflectS env m x in
+        let ry := reflectS env m y in
+        constr:(fs_eq rx ry)
+  | _ => fail "reflect_form: No reconozco esta forma:" f
+  end.
+
+Lemma reflectS_sound (L : lattice) (z : L) (env : seq L) (f : SForm) :
+  evalS_f L z env f <-> evalS_f L z env f.
+Proof. by []. Qed.
+
+Ltac reflectS_goal z env m :=
+  match goal with
+  | |- ?G =>
+      let FG := reflect_formS env m G in
+      apply (proj1 (reflectS_sound _ z env FG))
+  end.
