ProyectoCoq/Def_Lattice.v
@@ -1,0 +1,33 @@
+From mathcomp Require Import all_ssreflect.
+
+Definition reflexive {T : Type} (rel : T -> T -> Prop) : Prop := forall x :T, rel x x.
+Definition antisymetric {T : Type} (rel : T -> T -> Prop) : Prop := forall x y : T, (rel x y) -> (rel y x) -> (x = y).
+Definition transitive {T : Type} (rel : T -> T -> Prop) :Prop := forall x y z :T, rel x y -> rel y z -> rel x z.
+Definition order {T : Type} (rel : T -> T -> Prop) := reflexive rel /\ antisymetric rel /\ transitive rel.
+
+Structure ordenParcial := OrdenParcial
+  {
+    O :> Type;
+    ord : O -> O -> Prop;
+    reflexT : reflexive ord;
+    antisymT : antisymetric ord;
+    transT : transitive ord;
+  }.
+Notation "x ≤ y" := (ord _ x y) (at level 50).
+
+Structure lattice := Lattice 
+  { 
+    T :> ordenParcial;
+    joinT : T -> T -> T;
+    jHT : (forall z : T , forall x y : T,  (x ≤ z /\ y ≤ z) <->( joinT x y) ≤ z);
+    meetT : T -> T -> T;
+    mHT : (forall z : T , forall x y : T,  (z ≤ x /\ z ≤ y) <-> z ≤ ( meetT x y));
+  }.
+
+Notation "x ⊓ y" := (@meetT _ x y) (at level 50). (* \sqcap *)
+Notation "x ⊔ y" := (@joinT _ x y) (at level 50). (* \sqcup *)
+Notation reflex := (reflexT _).
+Notation antisym := (antisymT _).
+Notation trans := (transT _).
+Notation JH := (@jHT _).
+Notation MH := (@mHT _).
