ProyectoCoq/Dualidad.v
@@ -1,0 +1,281 @@
+From mathcomp Require Import all_ssreflect.
+From ProyectoCoq Require Import Def_Lattice.
+
+Definition dord {T : ordenParcial} (x y : T) := ord T y x.
+
+Lemma Dreflex {T : ordenParcial} : reflexive (@dord T).
+Proof.
+move: (reflexT T).
+by rewrite /reflexive /dord.
+Qed.
+
+Lemma Dantisym {T : ordenParcial} : antisymetric (@dord T).
+Proof.
+move: (antisymT T).
+rewrite /antisymetric /dord.
+move=> H x y H0 H1.
+by move: (H x y H1 H0).
+Qed.
+
+Lemma Dtrans {T : ordenParcial} : transitive (@dord T).
+Proof.
+move: (transT T).
+rewrite /transitive /dord.
+move=> H x y z H0 H1.
+by move: (H z y x H1 H0).
+Qed.
+
+Canonical Structure dual_ord T := OrdenParcial (O T) (dord) Dreflex Dantisym Dtrans.
+
+Canonical Structure dual_lattice_of (L : lattice) : lattice :=
+  Lattice
+    (dual_ord L) (meetT L) (fun z x y => mHT L z x y) (joinT L) (fun z x y => jHT L z x y).
+
+Inductive Term : Set :=
+| Var  : nat -> Term
+| Meet : Term -> Term -> Term
+| Join : Term -> Term -> Term.
+
+Fixpoint eval (L : lattice) (z : L) (env : seq L) (t : Term) : L :=
+  match t with
+  | Var n     => nth z env n
+  | Meet t1 t2 => @meetT L (eval L z env t1) (eval L z env t2)
+  | Join t1 t2 => @joinT L (eval L z env t1) (eval L z env t2)
+  end.
+
+Inductive Form : Set :=
+| f_leq  : Term -> Term -> Form
+| f_eq   : Term -> Term -> Form
+| f_neg  : Form -> Form
+| f_conj : Form -> Form -> Form
+| f_or   : Form -> Form -> Form
+| f_imp  : Form -> Form -> Form.
+
+Fixpoint eval_f (L : lattice) (z : L) (env : seq L) (f : Form) : Prop :=
+  match f with
+  | f_leq t1 t2 => (eval L z env t1) ≤ (eval L z env t2)
+  | f_eq t1 t2  => (eval L z env t1) = (eval L z env t2)
+  | f_neg f1     => ~ (eval_f L z env f1)
+  | f_conj f1 f2  => eval_f L z env f1 /\ eval_f L z env f2
+  | f_or f1 f2    => (eval_f L z env f1) \/ (eval_f L z env f2)
+  | f_imp f1 f2   =>  (eval_f L z env f1) -> (eval_f L z env f2)
+  end.
+
+Fixpoint dual_t (t : Term) : Term :=
+  match t with
+  | Var n => Var n
+  | Meet t1 t2 => Join (dual_t t1) (dual_t t2)
+  | Join t1 t2 => Meet (dual_t t1) (dual_t t2)
+  end.
+
+Fixpoint dual (f : Form) : Form :=
+  match f with
+  | f_leq t1 t2 => f_leq (dual_t t2) (dual_t t1)
+  | f_eq t1 t2  => f_eq (dual_t t1) (dual_t t2)
+  | f_neg f1     => f_neg (dual f1)
+  | f_conj f1 f2  => f_conj (dual f1) (dual f2)
+  | f_or f1 f2    => f_or (dual f1) (dual f2)
+  | f_imp f1 f2   => f_imp (dual f1) (dual f2)
+  end.
+
+(* Theorem eval_dual *)
+
+Lemma jldm : forall (L : lattice), joinT (dual_lattice_of L) = meetT L.
+Proof.
+  by [].
+Qed.
+
+Lemma mldj : forall (L : lattice), meetT (dual_lattice_of L) = joinT L.
+Proof.
+  by [].
+Qed.
+
+Lemma  eval_m : forall (L : lattice) (z : L) (env : seq L) (t0 t1 : Term), 
+              eval L z env (Meet t0 t1) = meetT L (eval L z env t0) (eval L z env t1).
+Proof. by move=> L0 env0; rewrite /eval. Qed.
+
+Lemma eval_j : forall (L : lattice) (z : L) (env : seq L) (t0 t1 : Term), 
+              eval L z env (Join t0 t1) = joinT L (eval L z env t0) (eval L z env t1).
+Proof. by move=> L0 env0; rewrite /eval. Qed.
+
+Lemma eval_conj : forall (L : lattice) (z : L) (env : seq L) (f0 f1 : Form), 
+                   eval_f L z env (f_conj f0 f1) = and (eval_f L z env f0) (eval_f L z env f1).
+Proof.  by []. Qed.
+
+Lemma dual_conj : forall (f0 f1 : Form), dual (f_conj f0 f1) = f_conj (dual f0) (dual f1).
+Proof.  by []. Qed.
+
+Lemma eval_or : forall (L : lattice) (z : L) (env : seq L) (f0 f1 : Form), 
+                   eval_f L z env (f_or f0 f1) = or (eval_f L z env f0) (eval_f L z env f1).
+Proof.  by []. Qed.
+
+Lemma dual_or : forall (f0 f1 : Form), dual (f_or f0 f1) = f_or (dual f0) (dual f1).
+Proof.  by []. Qed.
+
+Lemma eval_imp : forall (L : lattice) (z : L) (env : seq L) (f0 f1 : Form), 
+                   eval_f L z env (f_imp f0 f1) =(( eval_f L z env f0) -> (eval_f L z env f1)).
+Proof. by []. Qed.
+
+Lemma dual_imp : forall (f0 f1 : Form), dual (f_imp f0 f1) = f_imp (dual f0) (dual f1).
+Proof.  by []. Qed.
+
+Lemma dual_m : forall t0 t1 : Term, 
+                dual_t (Meet t0 t1) = Join (dual_t t0) (dual_t t1).
+Proof.  by move=> t2 t3; rewrite /dual_t. Qed.
+
+Lemma dual_j : forall t0 t1 : Term, 
+                dual_t (Join t0 t1) = Meet (dual_t t0) (dual_t t1).
+Proof.  by move=> t2 t3; rewrite /dual_t. Qed.
+
+Lemma le_dual (L : lattice) (x y : L) :
+  (ord (dual_lattice_of L) x y) <-> (ord L y x).
+Proof.
+by [].
+Qed.
+
+Theorem eval_dual (L : lattice) (z : L) (env : seq L) (t : Term) :
+  eval (dual_lattice_of L) z env t = eval L z env (dual_t t).
+Proof.
+elim t.
+  
+  (* Var n *)
+  move=> n0.
+  by rewrite  {1}/eval/dual_t/eval.
+  
+  (* Meet t0 t1*)
+  move=> t0 H0 t1 H1.
+  rewrite dual_m (eval_j L z env).
+  rewrite (eval_m (dual_lattice_of L) z env).
+  by rewrite H0 H1 mldj.
+
+  (* Join t0 t1 *)
+  move=> t0 H0 t1 H1.
+  rewrite dual_j (eval_m L z env).
+  rewrite (eval_j (dual_lattice_of L) z env).
+  by rewrite H0 H1 jldm.
+Qed.
+
+Theorem eval_dual_f (L : lattice) (z : L) (env : seq L) (f : Form) :
+  eval_f (dual_lattice_of L) z env f = eval_f L z env (dual f).
+Proof.
+elim f.
+  (* Term *)
+  move=> t0 t1.
+  by rewrite /dual /eval_f eval_dual eval_dual.
+  
+  move=> t0 t1.
+  by rewrite /dual /eval_f eval_dual eval_dual.
+  
+  (* Neg *)
+  move=> f0 H0.
+  have aux: forall (L : lattice) (z : L) (env : seq L) (f0 : Form), eval_f L z env (f_neg f0) = ~ (eval_f L z env f0).
+    by [].
+  have auxd: forall (f0 : Form), dual (f_neg f0) = f_neg (dual f0).
+    by [].
+  rewrite auxd aux aux.
+  by rewrite H0.
+
+  (* Conj *)
+  move=> f0 H0 f1 H1.
+  rewrite dual_conj eval_conj eval_conj.
+  by rewrite H0 H1.
+  
+  (* Or *)
+  move=> f0 H0 f1 H1.
+  rewrite dual_or eval_or eval_or.
+  by rewrite H0 H1.
+  
+  (* Imp *)
+  move=> f0 H0 f1 H1.
+  rewrite dual_imp eval_imp eval_imp.
+  by rewrite H0 H1.
+Qed.
+
+
+Lemma dual_td : forall t : Term, t = dual_t (dual_t t).
+Proof.
+move=> t; elim t.
+  by rewrite /dual_t.
+  
+  move=> t0 H0 t1 H1.
+  by rewrite dual_m dual_j -H0 -H1.
+  
+  move=> t0 H0 t1 H1.
+  by rewrite dual_j dual_m -H0 -H1.
+Qed.
+
+Lemma duald : forall F : Form, F = dual (dual F).
+Proof.
+move=>F; elim F.
+  by move=> t0 t1; rewrite /dual {1}(dual_td t0) {1}(dual_td t1).
+
+  by move=> t0 t1; rewrite /dual {1}(dual_td t0) {1}(dual_td t1).
+
+  by move=> F0 H0; rewrite {1}H0 {3 4}/dual.
+
+  by move=> F0 H0 F1 H1; rewrite dual_conj dual_conj -H0 -H1.
+
+  by move=> F0 H0 F1 H1; rewrite dual_or dual_or -H0 -H1.
+
+  by move=> F0 H0 F1 H1; rewrite dual_imp dual_imp -H0 -H1.
+Qed.
+
+Definition Teorema (F : Form) : Prop :=
+forall (L : lattice) (z : L) (env : seq L), (eval_f L z env F).
+
+Theorem Dualidad : forall f : Form, (Teorema f) -> (Teorema (dual f)).
+Proof.
+move=> f.
+elim f.
+  move=> t0 t1.
+
+    (* Caso: leq *)
+
+    rewrite /dual /Teorema => Hip L z env.
+    move: (Hip (dual_lattice_of L) z env).
+    by rewrite eval_dual_f /dual.
+
+    (* Caso: eq *)
+    
+    rewrite /Teorema /dual /eval_f => t0 t1 Hip L z env.
+    move: (Hip (dual_lattice_of L) z env).
+    by rewrite eval_dual eval_dual.
+
+    (* Caso: neg *)
+    rewrite /Teorema => f0 _ Hip L z env.
+    move: (Hip (dual_lattice_of L) z env).
+    have aux: forall (L : lattice) (z : L) (env : seq L) (f0 : Form), eval_f L z env (f_neg f0) = ~ (eval_f L z env f0).
+      by [].
+    have auxd: forall (f0 : Form), dual (f_neg f0) = f_neg (dual f0).
+      by [].
+    rewrite auxd aux aux.
+    by rewrite eval_dual_f.
+
+    (* Caso: Conj *)
+    rewrite /Teorema => f0 _ f1 _ Hip L z env.
+    move: (Hip (dual_lattice_of L) z env).
+    rewrite dual_conj eval_conj eval_conj.
+    by rewrite eval_dual_f eval_dual_f.
+
+    (* Caso: Or *)
+    rewrite /Teorema => f0 _ f1 _ Hip L z env.
+    move: (Hip (dual_lattice_of L) z env).
+    rewrite dual_or eval_or eval_or.
+    by rewrite eval_dual_f eval_dual_f.
+
+    (* Caso: Imp *)
+    rewrite /Teorema => f0 _ f1 _ Hip L z env.
+    move: (Hip (dual_lattice_of L) z env).
+    rewrite dual_imp eval_imp eval_imp.
+    by rewrite eval_dual_f eval_dual_f.
+Qed.
+(*    Fin del Teorema de dualidad     *)
+
+Lemma Dual : forall f : Form, (Teorema f) <-> (Teorema (dual f)).
+Proof.
+move=> f.
+split.
+  by move: (Dualidad f).
+move: (Dualidad (dual f))=> H.
+by rewrite {2}(duald f).
+Qed.
