ProyectoCoq/Dualidad_Bumcrot.v
@@ -1,0 +1,390 @@
+From mathcomp Require Import all_ssreflect.
+From ProyectoCoq Require Import Def_Lattice.
+From ProyectoCoq Require Import Dualidad.
+From ProyectoCoq Require Import MathCompLattices_SeqEnv.
+
+Structure bumcrotLattice := BumcrotLattice 
+  {
+    BumL :> boundedLattice;
+    Mod: (@Modu_L BumL)
+  }.
+
+Inductive TermB : Set :=
+| TopB : TermB
+| BotB : TermB
+| VarB  : nat -> TermB
+| MeetB : TermB -> TermB -> TermB
+| JoinB : TermB -> TermB -> TermB.
+
+Fixpoint evalB (L : bumcrotLattice) (z : L) (env : seq L) (t : TermB) : L :=
+  match t with
+  | TopB        => top
+  | BotB        => bot
+  | VarB n      => nth z env n
+  | MeetB t1 t2 => @meetT L (evalB L z env t1) (evalB L z env t2)
+  | JoinB t1 t2 => @joinT L (evalB L z env t1) (evalB L z env t2)
+  end.
+
+Inductive FormB : Set :=
+| fb_leq  : TermB -> TermB -> FormB
+| fb_eq   : TermB -> TermB -> FormB
+| fb_neg  : FormB -> FormB
+| fb_conj : FormB -> FormB -> FormB
+| fb_or   : FormB -> FormB -> FormB
+| fb_imp  : FormB -> FormB -> FormB.
+
+Fixpoint evalB_f (L : bumcrotLattice) (z : L) (env : seq L) (f : FormB) : Prop :=
+  match f with
+  | fb_leq t1 t2 => (evalB L z env t1) ≤ (evalB L z env t2)
+  | fb_eq t1 t2  => (evalB L z env t1) = (evalB L z env t2)
+  | fb_neg f1     => ~ (evalB_f L z env f1)
+  | fb_conj f1 f2  => evalB_f L z env f1 /\ evalB_f L z env f2
+  | fb_or f1 f2    => (evalB_f L z env f1) \/ (evalB_f L z env f2)
+  | fb_imp f1 f2   =>  (evalB_f L z env f1) -> (evalB_f L z env f2)
+  end.
+
+Fixpoint dualB_t (t : TermB) : TermB :=
+  match t with
+  | TopB  => BotB
+  | BotB  => TopB
+  | VarB n => VarB n
+  | MeetB t1 t2 => JoinB (dualB_t t1) (dualB_t t2)
+  | JoinB t1 t2 => MeetB (dualB_t t1) (dualB_t t2)
+  end.
+
+Fixpoint dualB (f : FormB) : FormB :=
+  match f with
+  | fb_leq t1 t2 => fb_leq (dualB_t t2) (dualB_t t1)
+  | fb_eq t1 t2  => fb_eq (dualB_t t1) (dualB_t t2)
+  | fb_neg f1     => fb_neg (dualB f1)
+  | fb_conj f1 f2  => fb_conj (dualB f1) (dualB f2)
+  | fb_or f1 f2    => fb_or (dualB f1) (dualB f2)
+  | fb_imp f1 f2   => fb_imp (dualB f1) (dualB f2)
+  end.
+
+Canonical Structure dual_bounded_lattice_of (L : boundedLattice) : boundedLattice :=
+  BoundedLattice
+    (dual_lattice_of L) (Bot L) (Top L)  (fun a => 
+      let '(conj Htop Hbot) := Top_Bottom L a in
+      conj Hbot Htop) .
+
+
+Lemma le_dualBound (L : boundedLattice) (x y : L) :
+  (ord (dual_bounded_lattice_of L) x y) <-> (ord L y x).
+Proof.
+by [].
+Qed.
+
+Lemma le_dualj (L : boundedLattice) (x y : L) :
+  (@joinT (dual_bounded_lattice_of L) x y) = (@meetT L x y).
+Proof.
+by [].
+Qed.
+
+Lemma le_dualm (L : boundedLattice) (x y : L) :
+  (@meetT (dual_bounded_lattice_of L) x y) = (@joinT L x y).
+Proof.
+by [].
+Qed.
+
+
+Lemma modular_dual (L : boundedLattice) (z : L) (P : @Modu_L L) : @Modu_L (dual_bounded_lattice_of L).
+Proof.
+  rewrite /Modu_L.
+  move=> p q r.
+  rewrite le_dualBound le_dualj le_dualj le_dualm le_dualm.
+  by move: ((@Modular2 L z P) r q p).
+Qed.
+
+Canonical Structure dual_bumcrot_lattice_of (B : bumcrotLattice) (z : B) : bumcrotLattice :=
+  BumcrotLattice
+    (dual_bounded_lattice_of B)
+    (modular_dual (B) z (Mod B)).
+
+
+Lemma jldmB : forall (L : bumcrotLattice) (z : L) , joinT (dual_bumcrot_lattice_of L z) = meetT L.
+Proof.
+  by [].
+Qed.
+
+Lemma mldjB : forall (L : bumcrotLattice) (z : L), meetT (dual_bumcrot_lattice_of L z) = joinT L.
+Proof.
+  by [].
+Qed.
+
+Lemma  evalB_m : forall (L : bumcrotLattice) (z : L) (env : seq L) (t0 t1 : TermB), 
+              evalB L z env (MeetB t0 t1) = meetT L (evalB L z env t0) (evalB L z env t1).
+Proof. by move=> L0 env0; rewrite /evalB. Qed.
+
+Lemma evalB_j : forall (L : bumcrotLattice) (z : L) (env : seq L) (t0 t1 : TermB), 
+              evalB L z env (JoinB t0 t1) = joinT L (evalB L z env t0) (evalB L z env t1).
+Proof. by move=> L0 env0; rewrite /evalB. Qed.
+
+Lemma evalB_conj : forall (L : bumcrotLattice) (z : L) (env : seq L) (f0 f1 : FormB), 
+                   evalB_f L z env (fb_conj f0 f1) = and (evalB_f L z env f0) (evalB_f L z env f1).
+Proof.  by []. Qed.
+
+Lemma dualB_conj : forall (f0 f1 : FormB), dualB (fb_conj f0 f1) = fb_conj (dualB f0) (dualB f1).
+Proof.  by []. Qed.
+
+Lemma evalB_or : forall (L : bumcrotLattice) (z : L) (env : seq L) (f0 f1 : FormB), 
+                   evalB_f L z env (fb_or f0 f1) = or (evalB_f L z env f0) (evalB_f L z env f1).
+Proof.  by []. Qed.
+
+Lemma dualB_or : forall (f0 f1 : FormB), dualB (fb_or f0 f1) = fb_or (dualB f0) (dualB f1).
+Proof.  by []. Qed.
+
+Lemma evalB_imp : forall (L : bumcrotLattice) (z : L) (env : seq L) (f0 f1 : FormB), 
+                   evalB_f L z env (fb_imp f0 f1) =(( evalB_f L z env f0) -> (evalB_f L z env f1)).
+Proof. by []. Qed.
+
+Lemma dualB_imp : forall (f0 f1 : FormB), dualB (fb_imp f0 f1) = fb_imp (dualB f0) (dualB f1).
+Proof.  by []. Qed.
+
+Lemma dualB_m : forall t0 t1 : TermB, 
+                dualB_t (MeetB t0 t1) = JoinB (dualB_t t0) (dualB_t t1).
+Proof.  by move=> t2 t3; rewrite /dualB_t. Qed.
+
+Lemma dualB_j : forall t0 t1 : TermB, 
+                dualB_t (JoinB t0 t1) = MeetB (dualB_t t0) (dualB_t t1).
+Proof.  by move=> t2 t3; rewrite /dualB_t. Qed.
+
+Theorem eval_dualB (L : bumcrotLattice) (z : L) (env : seq L) (t : TermB) :
+  evalB (dual_bumcrot_lattice_of L z) z env t = evalB L z env (dualB_t t).
+Proof.
+elim t.
+  (* TopB *)
+  by rewrite /evalB.
+  (* BotB *)
+  by rewrite /evalB.
+
+  (* VarB n *)
+  move=> n0.
+  by rewrite {1}/evalB/dualB_t/evalB.
+  
+  (* MeetB t0 t1*)
+  move=> t0 H0 t1 H1.
+  rewrite dualB_m (evalB_j L z env).
+  rewrite (evalB_m (dual_bumcrot_lattice_of L z) z env).
+  by rewrite H0 H1 mldjB.
+
+  (* JoinB t0 t1 *)
+  move=> t0 H0 t1 H1.
+  rewrite dualB_j (evalB_m L z env).
+  rewrite (evalB_j (dual_bumcrot_lattice_of L z) z env).
+  by rewrite H0 H1 jldmB.
+Qed.
+
+Lemma le_dualB (L : bumcrotLattice) (z : L) (x y : L) :
+  (ord (dual_bumcrot_lattice_of L z) x y) <-> (ord L y x).
+Proof.
+by [].
+Qed.
+
+Theorem evalB_dual_f (L : bumcrotLattice) (z : L) (env : seq L) (f : FormB) :
+  evalB_f (dual_bumcrot_lattice_of L z) z env f = evalB_f L z env (dualB f).
+Proof.
+elim f.
+  (* Term *)
+  move=> t0 t1.
+  by rewrite /dualB /evalB_f eval_dualB eval_dualB.
+  
+  move=> t0 t1.
+  by rewrite /dualB /evalB_f eval_dualB eval_dualB.
+  
+  (* Neg *)
+  move=> f0 H0.
+  have aux: forall (L : bumcrotLattice) (z : L) (env : seq L) (f0 : FormB), evalB_f L z env (fb_neg f0) = ~ (evalB_f L z env f0).
+    by [].
+  have auxd: forall (f0 : FormB), dualB (fb_neg f0) = fb_neg (dualB f0).
+    by [].
+  rewrite auxd aux aux.
+  by rewrite H0.
+
+  (* Conj *)
+  move=> f0 H0 f1 H1.
+  rewrite dualB_conj evalB_conj evalB_conj.
+  by rewrite H0 H1.
+  
+  (* Or *)
+  move=> f0 H0 f1 H1.
+  rewrite dualB_or evalB_or evalB_or.
+  by rewrite H0 H1.
+  
+  (* Imp *)
+  move=> f0 H0 f1 H1.
+  rewrite dualB_imp evalB_imp evalB_imp.
+  by rewrite H0 H1.
+Qed.
+
+
+Lemma dualB_td : forall t : TermB, t = dualB_t (dualB_t t).
+Proof.
+move=> t; elim t.
+  
+  by rewrite /dualB_t.
+  
+  by rewrite /dualB_t.
+
+  by rewrite /dualB_t.
+  
+  move=> t0 H0 t1 H1.
+  by rewrite dualB_m dualB_j -H0 -H1.
+  
+  move=> t0 H0 t1 H1.
+  by rewrite dualB_j dualB_m -H0 -H1.
+Qed.
+
+Lemma dualBd : forall F : FormB, F = dualB (dualB F).
+Proof.
+move=>F; elim F.
+  by move=> t0 t1; rewrite /dualB {1}(dualB_td t0) {1}(dualB_td t1).
+
+  by move=> t0 t1; rewrite /dualB {1}(dualB_td t0) {1}(dualB_td t1).
+
+  by move=> F0 H0; rewrite {1}H0 {3 4}/dualB.
+
+  by move=> F0 H0 F1 H1; rewrite dualB_conj dualB_conj -H0 -H1.
+
+  by move=> F0 H0 F1 H1; rewrite dualB_or dualB_or -H0 -H1.
+
+  by move=> F0 H0 F1 H1; rewrite dualB_imp dualB_imp -H0 -H1.
+Qed.
+
+
+
+Definition TeoremaB (F : FormB) : Prop :=
+forall (L : bumcrotLattice) (z : L) (env : seq L), (evalB_f L z env F).
+
+Theorem DualidadB : forall f : FormB, (TeoremaB f) -> (TeoremaB (dualB f)).
+Proof.
+move=> f.
+elim f.
+  move=> t0 t1.
+
+    (* Caso: leq *)
+
+    rewrite /dualB /TeoremaB => Hip L z env.
+    move: (Hip (dual_bumcrot_lattice_of L z) z env).
+    by rewrite evalB_dual_f /dualB.
+
+    (* Caso: eq *)
+    
+    rewrite /TeoremaB /dualB /evalB_f => t0 t1 Hip L z env.
+    move: (Hip (dual_bumcrot_lattice_of L z) z env).
+    by rewrite eval_dualB eval_dualB.
+
+    (* Caso: neg *)
+    rewrite /TeoremaB => f0 _ Hip L z env.
+    move: (Hip (dual_bumcrot_lattice_of L z) z env).
+    have aux: forall (L : bumcrotLattice) (z : L) (env : seq L) (f0 : FormB), evalB_f L z env (fb_neg f0) = ~ (evalB_f L z env f0).
+      by [].
+    have auxd: forall (f0 : FormB), dualB (fb_neg f0) = fb_neg (dualB f0).
+      by [].
+    rewrite auxd aux aux.
+    by rewrite evalB_dual_f.
+
+    (* Caso: Conj *)
+    rewrite /TeoremaB => f0 _ f1 _ Hip L z env.
+    move: (Hip (dual_bumcrot_lattice_of L z) z env).
+    rewrite dualB_conj evalB_conj evalB_conj.
+    by rewrite evalB_dual_f evalB_dual_f.
+
+    (* Caso: Or *)
+    rewrite /TeoremaB => f0 _ f1 _ Hip L z env.
+    move: (Hip (dual_bumcrot_lattice_of L z) z env).
+    rewrite dualB_or evalB_or evalB_or.
+    by rewrite evalB_dual_f evalB_dual_f.
+
+    (* Caso: Imp *)
+    rewrite /TeoremaB => f0 _ f1 _ Hip L z env.
+    move: (Hip (dual_bumcrot_lattice_of L z) z env).
+    rewrite dualB_imp evalB_imp evalB_imp.
+    by rewrite evalB_dual_f evalB_dual_f.
+Qed.
+(*    Fin del Teorema de dualidad para lattices acotadas     *)
+
+Lemma DualB : forall f : FormB, (TeoremaB f) <-> (TeoremaB (dualB f)).
+Proof.
+move=> f.
+split.
+  by move: (DualidadB f).
+move: (DualidadB (dualB f))=> H.
+by rewrite {2}(dualBd f).
+Qed.
+
+
+(* Ltac para Bumcrot *)
+
+Ltac rankB env n v :=
+  match env with
+  | (cons ?X1 ?X2) =>
+      let env' := constr:(X2) in
+        match constr:(X1 = v) with
+        | (?X1 = ?X1) => n
+        | _ => rankB env' (S n) v
+        end
+  end.
+
+Ltac reflectB env m j v :=
+  match v with
+  | (m _ ?X1 ?X2) =>
+      let r1 := reflectB env m j X1
+      with r2 := reflectB env m j X2 in
+        constr:(MeetB r1 r2)
+  | (j _ ?X1 ?X2) =>
+      let r1 := reflectB env m j X1
+      with r2 := reflectB env m j X2 in
+        constr:(JoinB r1 r2)
+  | ?X1 =>
+      let n := rankB env 0 X1 in
+        constr:(VarB n)
+  | top => constr:(TopB)
+  | bot => constr:(BotB)
+  | _ => constr:(VarB 0)
+  end.
+
+Ltac reflect_formB env m j f :=
+  lazymatch f with
+  | ?x ≤ ?y =>
+        let rx := reflectB env m j x in
+        let ry := reflectB env m j y in
+        constr:(fb_leq rx ry)
+  | ?x = ?y =>
+        let rx := reflectB env m j x in
+        let ry := reflectB env m j y in
+        constr:(fb_eq rx ry)
+  | ~ ?p =>
+        let rp := reflect_formB env m j p in
+        constr:(fb_neg rp)
+  | ?p /\ ?q =>
+        let rp := reflect_formB env m j p in
+        let rq := reflect_formB env m j q in
+        constr:(fb_conj rp rq)
+  | ?p \/ ?q =>
+        let rp := reflect_formB env m j p in
+        let rq := reflect_formB env m j q in
+        constr:(fb_or rp rq)
+  | ?p -> ?q =>
+        let rp := reflect_formB env m j p in
+        let rq := reflect_formB env m j q in
+        constr:(fb_imp rp rq)
+  | _ => fail "reflect_form: No reconozco esta forma:" f
+  end.
+
+Lemma reflect_sound_fullB (L : bumcrotLattice) (z : L) (env : seq L) (f : FormB) :
+  evalB_f L z env f <-> evalB_f L z env f.
+Proof. by []. Qed.
+
+Ltac reflectB_goal z env m j :=
+  match goal with
+  | |- ?G =>
+      let FG := reflect_formB env m j G in
+      apply (proj1 (reflect_sound_fullB _ z env FG))
+  end.
+
+Lemma reflectDualB (L : bumcrotLattice) (z : L) (env : seq L) (F : FormB) : TeoremaB (F) -> evalB_f L z env F.
+Proof.
+rewrite /TeoremaB=> H.
+by move: (H L z env).
+Qed.
