ProyectoCoq/Ltac_Dual.v
@@ -1,0 +1,74 @@
+From mathcomp Require Import all_ssreflect.
+From ProyectoCoq Require Import Def_Lattice.
+From ProyectoCoq Require Import Dualidad.
+
+Ltac rank env n v :=
+  match env with
+  | (cons ?X1 ?X2) =>
+      let env' := constr:(X2) in
+        match constr:(X1 = v) with
+        | (?X1 = ?X1) => n
+        | _ => rank env' (S n) v
+        end
+  end.
+
+Ltac reflect env m j v :=
+  match v with
+  | (m _ ?X1 ?X2) =>
+      let r1 := reflect env m j X1
+      with r2 := reflect env m j X2 in
+        constr:(Meet r1 r2)
+  | (j _ ?X1 ?X2) =>
+      let r1 := reflect env m j X1
+      with r2 := reflect env m j X2 in
+        constr:(Join r1 r2)
+  | ?X1 =>
+      let n := rank env 0 X1 in
+        constr:(Var n)
+  | _ => constr:(Var 0)
+  end.
+
+Ltac reflect_form env m j f :=
+  lazymatch f with
+  | ?x ≤ ?y =>
+        let rx := reflect env m j x in
+        let ry := reflect env m j y in
+        constr:(f_leq rx ry)
+  | ?x = ?y =>
+        let rx := reflect env m j x in
+        let ry := reflect env m j y in
+        constr:(f_eq rx ry)
+  | ~ ?p =>
+        let rp := reflect_form env m j p in
+        constr:(f_neg rp)
+  | ?p /\ ?q =>
+        let rp := reflect_form env m j p in
+        let rq := reflect_form env m j q in
+        constr:(f_conj rp rq)
+  | ?p \/ ?q =>
+        let rp := reflect_form env m j p in
+        let rq := reflect_form env m j q in
+        constr:(f_or rp rq)
+  | ?p -> ?q =>
+        let rp := reflect_form env m j p in
+        let rq := reflect_form env m j q in
+        constr:(f_imp rp rq)
+  | _ => fail "reflect_form: No reconozco esta forma:" f
+  end.
+
+Lemma reflect_sound_full (L : lattice) (z : L) (env : seq L) (f : Form) :
+  eval_f L z env f <-> eval_f L z env f.
+Proof. by []. Qed.
+
+Ltac reflect_goal z env m j :=
+  match goal with
+  | |- ?G =>
+      let FG := reflect_form env m j G in
+      apply (proj1 (reflect_sound_full _ z env FG))
+  end.
+
+Lemma reflectDual (L : lattice) (z : L) (env : seq L) (F : Form) : Teorema (F) -> eval_f L z env F.
+Proof.
+rewrite /Teorema=> H.
+by move: (H L z env).
+Qed.
