ProyectoCoq/MathCompLattices_SeqEnv.v
@@ -1,0 +1,658 @@
+From mathcomp Require Import all_ssreflect.
+From ProyectoCoq Require Import Def_Lattice.
+From ProyectoCoq Require Import Dualidad.
+From ProyectoCoq Require Import Ltac_Dual.
+From Coq Require Import Logic.
+
+
+Lemma dobl (A : Prop) :  A <-> A /\ A.
+Proof.
+split. by [].
+move=> [h1 h2]; by [].
+Qed.
+
+Lemma ab_leq_jab {T : lattice} (z : T) : forall a b : T ,   a ≤ (a ⊔ b) /\  b ≤ (a ⊔ b).
+Proof.
+move=> a b.
+split.
+  by move: (reflex (a ⊔ b)); rewrite -(JH (a ⊔ b) a b) => /proj1.
+by move: (reflex (a ⊔ b)); rewrite -(JH (a ⊔ b) a b) => /proj2.
+Qed.
+
+Lemma mab_leq_ab {T : lattice} (z : T) : forall a b : T ,  (a ⊓ b) ≤ a /\ (a ⊓ b) ≤ b.
+Proof.
+(* Prueba por dualidad *)
+move=> a b.
+reflect_goal z [:: a; b] meetT joinT.
+apply reflectDual.
+rewrite Dual/dual/dual_t/Teorema => L0 z0 env0.
+rewrite /eval_f.
+by move: ((@ab_leq_jab L0 z0) (eval L0 z0 env0 (Var 0)) (eval L0 z0 env0 (Var 1)) ).
+Qed.
+
+Lemma ConnectJ {T : lattice} (z : T) : forall a b : T ,  a ≤ b <-> (a ⊔ b = b).
+Proof.
+split.
+move=> abLeq.
+  apply: antisym.
+    rewrite -(JH).
+    split.
+      by [].
+    by apply: reflex.
+  move: (reflex (a ⊔ b)).
+  by rewrite -(JH) => /proj2.
+move=> H.
+move: (reflex (a ⊔ b)).
+rewrite {2}H.
+move: (ab_leq_jab z a b) => /proj1.
+by apply: trans.
+Qed.
+
+Lemma ConnectM {T : lattice} (z : T) : forall a b : T , a ≤ b <-> (b ⊓ a = a).
+Proof.
+move=> a b; rewrite /iff.
+(* Prueba por dualidad *)
+reflect_goal z [:: a; b] meetT joinT.
+apply reflectDual.
+rewrite Dual /dual /dual_t => L0 z0 env0.
+rewrite /eval_f.
+move: ((@ConnectJ L0 z0 ) (eval L0 z0 env0 (Var 1)) (eval L0 z0 env0 (Var 0)) ).
+by rewrite /iff.
+Qed.
+
+(* Propiedades L1 a L4*)
+
+Lemma L3 {T : lattice} (z : T) : forall a : T , a ⊔ a = a.
+Proof.
+move=> a.
+move: (reflex  a). 
+by move=> /(ConnectJ z).
+Qed.
+
+Lemma L3d {T : lattice} (z : T) : forall a : T , a ⊓ a = a.
+Proof.
+move=> a.
+(* Prueba por dualidad *)
+reflect_goal z [:: a] meetT joinT.
+apply reflectDual.
+rewrite Dual /dual /dual_t => L0 z0 env0.
+rewrite /eval_f.
+by move: ((@L3 L0 z0) (eval L0 z0 env0 (Var 0)) ).
+Qed.
+
+Lemma L2 {T : lattice} (z : T) : forall a b : T , a ⊔ b = b ⊔ a.
+Proof.
+move=> a b.
+apply: antisym.
+  move: (ab_leq_jab z b a) => /and_comm.
+  by rewrite JH. 
+move: (ab_leq_jab z a b) => /and_comm.
+by rewrite JH.
+Qed.
+
+Lemma L2d {T : lattice} (z : T) : forall a b : T , a ⊓ b = b ⊓ a.
+Proof.
+move=> a b.
+(* Prueba por dualidad *)
+reflect_goal z [:: a; b] meetT joinT.
+apply reflectDual.
+rewrite Dual /dual /dual_t => L0 z0 env0.
+rewrite /eval_f.
+by move: ((@L2 L0 z0) (eval L0 z0 env0 (Var 0)) (eval L0 z0 env0 (Var 1)) ).
+Qed.
+
+Lemma L4 {T : lattice} (z : T) : forall a b : T , a ⊔ (a ⊓ b) = a.
+Proof.
+move=> a b.
+move: (mab_leq_ab z a b) => /proj1.
+move=> /(ConnectJ z).
+by rewrite L2.
+Qed.
+
+Lemma L4d {T : lattice} (z : T) : forall a b : T , a ⊓ (a ⊔ b) = a.
+Proof.
+move=> a b.
+(* Prueba por dualidad *)
+reflect_goal z [:: a; b] meetT joinT.
+apply reflectDual.
+rewrite Dual /dual /dual_t => L0 z0 env0.
+rewrite /eval_f.
+by move: ((@L4 L0 z0) (eval L0 z0 env0 (Var 0)) (eval L0 z0 env0 (Var 1)) ).
+Qed.
+
+Lemma L1 {T : lattice} (z : T) : forall a b c : T , (a ⊔ b) ⊔ c = a ⊔ (b ⊔ c).
+Proof. 
+have c_leq_jab: forall x y w : T , w ≤ y -> w ≤ (x ⊔ y).
+    move=> x y w w_leq_y; move: (ab_leq_jab z x y) => /proj2.
+    move: w_leq_y; by apply: trans.
+move=> a b c.
+apply: antisym.
+  rewrite -JH.
+  split.
+    rewrite -JH.
+    split.
+      by move: (ab_leq_jab z a (b ⊔ c)) => /proj1. (*1° caso a ≤ sup a (sup b c)*)
+    by move: (ab_leq_jab z b c) => /proj1 /c_leq_jab. (*2° caso b ≤ sup a (sup b c)*)
+  by move: (ab_leq_jab z b c) => /proj2 /c_leq_jab. (*c ≤ sup a (sup b c)*)
+rewrite -JH.
+split.
+  rewrite (L2 z).
+  move: (ab_leq_jab z a b) => /proj1.
+  by move=> /c_leq_jab.
+rewrite -JH.
+split.
+  move: (ab_leq_jab z a b) => /proj2; rewrite [_ ⊔ c](L2 z).
+  by move=> /c_leq_jab.  (*sup c (sup a b)*)
+by move: (ab_leq_jab z (a ⊔ b) c) => /proj2. (*c ≤ sup (sup a b) c*)
+Qed.
+
+Lemma L1d {T : lattice} (z : T) : forall a b c : T , (a ⊓ b) ⊓ c = a ⊓ (b ⊓ c).
+Proof. 
+move=> a b c.
+(* Prueba por dualidad *)
+reflect_goal z [:: a; b; c] meetT joinT.
+apply reflectDual.
+rewrite Dual /dual /dual_t => L0 z0 env0.
+rewrite /eval_f.
+by move: ((@L1 L0 z0) (eval L0 z0 env0 (Var 0)) (eval L0 z0 env0 (Var 1))
+                      (eval L0 z0 env0 (Var 2)) ).
+Qed.
+
+Structure latticeAlg := LatticeAlg 
+  {
+    A :> Type;
+    j : A -> A -> A;
+    m : A -> A -> A;
+    l1 : forall a b c : A, j (j a b) c = j a (j b c);
+    l1d : forall a b c : A, m (m a b) c = m a (m b c);
+    l2 : forall a b : A, j a b = j b a;
+    l2d : forall a b : A, m a b = m b a;
+    l3 : forall a : A, j a a = a;
+    l3d : forall a : A, m a a = a;
+    l4 : forall a b : A, j a (m a b) = a;
+    l4d : forall a b : A, m a (j a b) = a
+  }.
+Notation "x ∧ y" := (@m _ x y) (at level 50). (* \wedge *)
+Notation "x ∨ y" := (@j _ x y) (at level 50). (* \vee *)
+Notation L1_Alg := (l1 _).
+Notation L1d_Alg := (l1d _).
+Notation L2_Alg := (l2 _).
+Notation L2d_Alg := (l2d _).
+Notation L3_Alg := (l3 _).
+Notation L3d_Alg := (l3d _).
+Notation L4_Alg := (l4 _).
+Notation L4d_Alg := (l4d _).
+
+Canonical Alg_lattice {T : lattice} (z : T) := LatticeAlg T (@joinT T) (@meetT T) (L1 z) (L1d z) (L2 z) (L2d z) (L3 z) (L3d z) (L4 z) (L4d z).
+
+Lemma AlgToSet1 {T : latticeAlg} : forall a b : T, ( a ∨ b = b) <-> ( a ∧ b = a).
+Proof.
+split.
+  move=> jab_b.
+  move: (L4d_Alg a b).
+  by rewrite jab_b.
+move=> mab_a.
+move: (L4_Alg b a).
+by rewrite L2d_Alg mab_a L2_Alg.
+Qed.
+
+Definition nord {T : latticeAlg} (a b : T) := (a ∨ b = b).
+Notation "x ≼ y" := (@nord _ x y) (at level 50). (* \preccurlyeq *)
+
+Lemma AlgToSetReflex {T : latticeAlg} : reflexive (@nord T).
+Proof.
+  move=> a.
+  rewrite /nord.
+  by apply: L3_Alg.
+Qed.
+
+Lemma AlgToSetAntisym {T : latticeAlg} : antisymetric (@nord T).
+Proof.
+  move=> a b.
+  rewrite /nord => supb.
+  by rewrite L2_Alg supb.
+Qed.
+
+Lemma AlgToSetTrans {T : latticeAlg} : transitive (@nord T).
+Proof.
+move=> a b c.
+rewrite /nord.
+move=> supab supbc.
+by move: (L1_Alg a b c); rewrite supab supbc.
+Qed.
+
+Canonical T_ordenParcial {T : latticeAlg} := OrdenParcial T (@nord T) AlgToSetReflex AlgToSetAntisym AlgToSetTrans.
+
+
+Lemma AlgToSet_joinAlg {T : latticeAlg} : forall z : T, (forall x y : T, (x ≼ z /\ y ≼ z) <-> (x ∨ y) ≼ z).
+Proof.
+move=> z x y.
+split.
+  rewrite /nord.
+  move=> [supxz supyz].
+  by move: supxz; rewrite -{1}(supyz) -L1_Alg.
+move=> H1.
+have cotaS: forall a b : T, (a ≼ (a ∨ b)) /\ (b ≼ (a ∨ b)).
+  move=> a b.
+  split.
+    by rewrite /nord -L1_Alg L3_Alg.
+  by rewrite /nord L2_Alg L1_Alg L3_Alg.
+split.
+  move: (cotaS x y) H1 => /proj1.
+  by apply: AlgToSetTrans.
+move: H1; move: (cotaS x y); move=> /proj2.
+by apply: AlgToSetTrans.
+Qed.
+
+Lemma AlgToSet_meetAlg {T : latticeAlg}: forall z : T, (forall x y : T, (z ≼ x /\ z ≼ y) <-> z ≼ (x ∧ y) ).
+Proof.
+move=> z x y.
+split.
+  rewrite /nord.
+  move => [/(AlgToSet1)-H1 /(AlgToSet1)-H2].
+  rewrite AlgToSet1.
+  move: H1.
+  by rewrite -{1}(H2) L1d_Alg (L2d_Alg y x).
+move=> H1.
+have cotaI: forall a b : T, ((a ∧ b) ≼ a) /\ ((a ∧ b) ≼ b).
+  move=> a b.
+  split.
+    by rewrite /nord AlgToSet1 (L2d_Alg) -(L1d_Alg) L3d_Alg.
+  by rewrite /nord AlgToSet1 L1d_Alg L3d_Alg.
+split.
+  move: (cotaI x y) => /proj1; move: H1. 
+  by apply: AlgToSetTrans.
+move: (cotaI x y) => /proj2; move: H1.
+by apply: AlgToSetTrans.
+Qed.
+
+Canonical T_lattice {T : latticeAlg} := Lattice (OrdenParcial T nord AlgToSetReflex AlgToSetAntisym AlgToSetTrans)
+                       (@j _) AlgToSet_joinAlg (@m _) AlgToSet_meetAlg.
+
+Lemma join_eq {T : latticeAlg}: forall a b : T,  a ∨ b = joinT T_lattice a b.
+Proof. by []. Qed.
+
+Lemma meet_eq {T : latticeAlg}: forall a b : T, a ∧ b = meetT T_lattice a b.
+Proof. by []. Qed.
+
+(* Proposición 2.19 *)
+
+Definition ordPreserv {L K : lattice} {f : L -> K} 
+                      := forall a b : L, a ≤ b -> (f a) ≤ (f b).
+
+Definition ordEmmbed {L K : lattice} {f : L -> K}
+                     := forall a b : L, a ≤ b <-> (f a) ≤ (f b).
+
+Definition Biyective {L K : lattice} {f : L -> K}
+                     := (forall a b : L, (f a) = (f b) <-> a = b) /\ (forall b : K, (exists a : L, b = f a )).
+
+Definition ordIso {L K : lattice} {f : L -> K} := (@Biyective L K f) /\ (@ordEmmbed L K f) .
+
+Definition joinOrdPreserv {L K : lattice} {f : L -> K}
+                          := forall x y : L, (f x) ⊔ (f y) ≤ f (x ⊔ y) .
+
+Definition meetOrdPreserv {L K : lattice} {f : L -> K}
+                          := forall x y : L, f (x ⊓ y) ≤ ((f x) ⊓ (f y)).
+
+Definition joinPreserv {L K : lattice} {f : L -> K}
+                       := forall x y : L, (f x) ⊔ (f y) = f (x ⊔ y).
+
+Definition meetPreserv {L K : lattice} {f : L -> K}
+                       := forall x y : L, f (x ⊓ y) = (f x) ⊓ (f y).
+
+Definition latticeIso {L K : lattice} {f : L -> K}
+                      := (@joinPreserv L K f) /\ (@meetPreserv L K f) /\ (@Biyective L K f).
+
+Lemma prop219i1 {L K : lattice} (z : L) (fz : K) {f : L -> K} : (@ordPreserv L K f)  <-> (@joinOrdPreserv L K f).
+Proof.
+split.
+  rewrite /ordPreserv => ordenP.
+  move=> a b.
+  move: (ab_leq_jab z a b) => [/(ordenP)-cota_fa /(ordenP)-cota_fb].
+  rewrite -JH.
+  by split.
+rewrite /joinOrdPreserv => H.
+move=> a b /(ConnectJ z)-jab_L.
+move: (H a b); rewrite jab_L.
+move: (ab_leq_jab fz (f a) (f b)) => /proj1.
+by apply: trans.
+Qed.
+
+
+Lemma prop219i2 {L K : lattice} (z : L) (fz : K) {f : L -> K} : (@ordPreserv L K f) <-> (@meetOrdPreserv L K f).
+Proof.
+split.
+  rewrite /ordPreserv => ordenP.
+  move=> a b.
+  move: (mab_leq_ab z a b) => [/ordenP-cota_fa /ordenP-cota_fb].
+  move: (conj cota_fa cota_fb).
+  by rewrite MH.
+rewrite /meetOrdPreserv => H.
+move=> a b /(ConnectM z); rewrite (L2d z) => mab_L.
+move: (mab_leq_ab fz (f a) (f b)) => /proj2.
+move: (H a b); rewrite mab_L.
+by apply: trans.
+Qed.
+
+Lemma prop219i3 {L K : lattice} (z : L) (fz : K) {f : L -> K} : (@ordIso L K f) <-> (@latticeIso L K f).
+Proof.
+split.
+  rewrite /ordIso /ordEmmbed /Biyective; move=> [[inj sob] H].
+  rewrite /latticeIso. 
+  split.
+    move=> x y; apply: antisym.
+      move: (@prop219i1 L K z fz f); rewrite /ordPreserv /joinOrdPreserv => /proj1-H2.
+      apply: H2 => c d.
+      by move: (H c d) => /proj1.
+    move: (sob ((f x) ⊔ (f y))) => [a Ha].
+    move: (ab_leq_jab fz (f x) (f y)).
+    rewrite Ha; move=> [/H-xleqa /H-yleqa].
+    by rewrite -H -JH.
+  split.
+    move=> x y; apply: antisym.
+      move: (@prop219i2 L K z fz f); rewrite /ordPreserv /meetOrdPreserv => /proj1-H2.
+      apply: H2 => c d;
+      by move: (H c d) => /proj1.
+      move: (sob ((f x) ⊓ (f y))) => [a Ha].
+      move: (mab_leq_ab fz (f x) (f y)).
+      rewrite Ha; move=> [/H-aleqx /H-aleqy].
+      by rewrite -H -MH.
+    by [].
+rewrite /latticeIso; move=> [Hjoin [Hmeet [inj sob]]].
+split.
+  by [].
+move=> a b.
+split.
+  by move=> /(ConnectJ z) /inj; rewrite -Hjoin -(ConnectJ).
+by rewrite (ConnectJ fz) Hjoin inj -(ConnectJ).
+Qed.
+
+(* Lattices modulares, distributivas y booleanas *)
+
+Lemma Lema4_1i {T : lattice} (z : T) : forall a b c : T, ((a ⊓ b) ⊔ (a ⊓ c)) ≤ (a ⊓ (b ⊔ c)).
+Proof.
+move=> a b c.
+rewrite -MH.
+split.
+  rewrite -JH.
+  split.
+    by move: (mab_leq_ab z a b) => /proj1.
+  by move: (mab_leq_ab z a c) => /proj1.
+rewrite -JH.
+move: (ab_leq_jab z b c) => [cota_b cota_c].
+split.
+  move: (mab_leq_ab z a b) cota_b => /proj2.
+  by apply: trans.
+move: (mab_leq_ab z a c) cota_c => /proj2.
+by apply: trans.
+Qed.
+
+Lemma Lema4_1id {T : lattice} (z : T) : forall a b c : T, (a ⊔ (b ⊓ c)) ≤ ((a ⊔ b) ⊓ (a ⊔ c)).
+Proof.
+move=> a b c.
+(* Prueba por dualidad *)
+reflect_goal z [:: a; b; c] meetT joinT.
+apply reflectDual.
+rewrite Dual /dual /dual_t => L0 z0 env0.
+rewrite /eval_f.
+by move: ((@Lema4_1i L0 z0) (eval L0 z0 env0 (Var 0)) (eval L0 z0 env0 (Var 1))
+           (eval L0 z0 env0 (Var 2)) ).
+Qed.
+
+Lemma Lema4_1ii {T : lattice} (z : T) : forall a b c : T, c ≤ a -> ((a ⊓ b) ⊔ c) ≤ (a ⊓ (b ⊔ c)).
+Proof.
+move=> a b c /ConnectM- H.
+by move: (Lema4_1i z a b c); rewrite H.
+Qed.
+
+Lemma Lema4_1iid {T : lattice} (z : T) : forall a b c : T, a ≤ c -> (a ⊔ (b ⊓ c)) ≤ ((a ⊔ b) ⊓ c).
+Proof.
+move=> a b c.
+(* Prueba por dualidad *)
+reflect_goal z [:: a; b; c] meetT joinT.
+apply reflectDual.
+rewrite Dual /dual /dual_t => L0 z0 env0.
+rewrite /eval_f.
+by move: ((@Lema4_1ii L0 z0) (eval L0 z0 env0 (Var 0)) (eval L0 z0 env0 (Var 1))
+           (eval L0 z0 env0 (Var 2)) ).
+Qed.
+
+Lemma Lema4_1iii {T : lattice} (z : T) : forall a b c : T, ((a ⊓ b) ⊔ (b ⊓ c) ⊔ (c ⊓ a)) ≤ ((a ⊔ b) ⊓ (b ⊔ c) ⊓ (c ⊔ a)).
+Proof.
+have aux : forall a b c : T, (a ⊓ b) ≤ (c ⊔ a).
+  move=> a b c; move: (ab_leq_jab z c a)=> /proj2.
+  move: (mab_leq_ab z a b) => /proj1.
+  by apply: trans.
+move=> a b c.
+rewrite -JH.
+split.
+  rewrite -MH.
+  split.
+    have H1 : b ≤ ((a ⊔ b) ⊓ (b ⊔ c)).
+      rewrite -MH.
+      split.
+        by move: (ab_leq_jab z a b) => /proj2.
+      by move: (ab_leq_jab z b c) => /proj1.
+    have H2 : ((a ⊓ b) ⊔ (b ⊓ c)) ≤ b.
+      rewrite -JH.
+      split.
+        by move: (mab_leq_ab z a b) => /proj2.
+      by move: (mab_leq_ab z b c) => /proj1.
+    by move: H1; move: H2; apply: trans.
+  rewrite -JH.
+  split.
+    by apply: aux.
+  by rewrite (L2d z) (L2 z); apply aux.
+rewrite -MH.
+split.
+  rewrite -MH.
+  split.
+    by rewrite (L2d z) (L2 z); apply aux.
+  by apply: aux.
+by rewrite (L2 z); apply: aux.
+Qed.
+
+
+Lemma Lema4_2i {T : lattice} (z : T) : forall a b c : T, (c ≤ a -> (a ⊓ (b ⊔ c)) = ((a ⊓ b) ⊔ c)) <->
+                                   (c ≤ a -> (a ⊓ (b ⊔ c)) = ((a ⊓ b) ⊔ (a ⊓ c))).
+Proof.
+split. 
+  by move=> H1 /dobl [/(ConnectM z)-H] /H1; rewrite H.
+by move=> H1 /dobl [/(ConnectM z)-H] /H1; rewrite H.
+Qed.
+
+Lemma Lema4_2ii {T : lattice} (z : T) : (forall a b c : T, c ≤ a -> (a ⊓ (b ⊔ c)) = ((a ⊓ b) ⊔ (a ⊓ c))) <->
+                  (forall p q r : T, (p ⊓ (q ⊔ (p ⊓ r))) = ((p ⊓ q) ⊔ (p ⊓ r))).
+Proof.
+split.
+  move=> H p q r.
+  move: (mab_leq_ab z p r) => /proj1.
+  rewrite (Lema4_2i z).
+  by apply: H.
+move=> H a b c /(ConnectM z)-cleqa.
+rewrite -{1}cleqa. 
+by apply: H.
+Qed.
+
+Lemma Lema4_3 {T : lattice} (z : T) : (forall a b c : T, (a ⊓ (b ⊔ c)) = (a ⊓ b) ⊔ (a ⊓ c)) <-> 
+                (forall p q r : T, (p ⊔ (q ⊓ r)) = (p ⊔ q) ⊓ (p ⊔ r)).
+Proof.
+split.
+  move=> H p q r.
+  move: (H (p ⊔ q) p r).
+  rewrite [(p ⊔ q) ⊓ p](L2d z) [p ⊓ (p ⊔ q)](L4d z) [(p ⊔ q) ⊓ r](L2d z).
+  rewrite (H r p q).
+  by rewrite -(L1 z) [r ⊓ p](L2d z) [p ⊔ (p ⊓ r)](L4 z) [r ⊓ q](L2d z).
+move=> H a b c.
+move: (H (a ⊓ b) a c).
+rewrite [(a ⊓ b) ⊔ a](L2 z) [a ⊔ (a ⊓ b)](L4 z).
+rewrite [(a ⊓ b) ⊔ c](L2 z) (H c a b).
+by rewrite -(L1d z) [c ⊔ a](L2 z) [a ⊓ (a ⊔ c)](L4d z) [c ⊔ b](L2 z).
+Qed.
+
+Definition Distributive {T : lattice} := forall a b c : T, (a ⊓ (b ⊔ c)) = ((a ⊓ b) ⊔ (a ⊓ c)).
+
+Definition Modu_L {T : lattice} := forall a b c : T, (c ≤ a -> (c ⊔ (b ⊓ a)) = ((c ⊔ b) ⊓ a)).
+
+Lemma Modular2 {T : lattice} (z : T) : (@Modu_L T) -> (forall a b c : T, (c ≤ a -> (a ⊓ (b ⊔ c)) = ((a ⊓ b) ⊔ c))).
+Proof.
+rewrite /Modu_L => H a b c.
+move=> /(H a b c).
+by rewrite (L2 z) [b ⊓_](L2d z) [_ ⊓ a](L2d z) [c ⊔ _](L2 z).
+Qed.
+
+Lemma ModularD {T : lattice} (z : T) : (@Modu_L T) -> (forall a b c : T, (a ≤ c -> (a ⊔ (b ⊓ c)) = ((a ⊔ b) ⊓ c)) ).
+Proof.
+rewrite /Modu_L => H a b c.
+by move=>/(H c b a).
+Qed.
+
+Lemma ModularD2 {T : lattice} (z : T) : (forall a b c : T, (a ≤ c -> (a ⊔ (b ⊓ c)) = ((a ⊔ b) ⊓ c)))
+                -> (forall a b c : T, (a ≤ c -> ( c ⊓ (b ⊔ a)  = (c ⊓ b) ⊔ a ))).
+Proof.
+move=> H a b c.
+move=> /(H _ b).
+by rewrite (L2 z) [b ⊓ c](L2d z) [_ ⊓ c](L2d z) [a ⊔ b](L2 z).
+Qed.
+
+Structure boundedLattice := BoundedLattice 
+  {
+    BL :> lattice;
+    Top : BL;
+    Bot : BL;
+    Top_Bottom : forall a : BL, a ≤ Top /\ Bot ≤ a
+  }.
+Notation  top := (Top _).
+Notation  bot := (Bot _).
+Notation TB := (Top_Bottom _).
+
+Structure booleanLattice := BooleanLattice
+  {
+    BooL :> boundedLattice;
+    Distr: (@Distributive BooL);
+    ExComplement : forall a : BooL, (exists b, (a ⊔ b = top ) /\ (a ⊓ b = bot) ) 
+  }.
+Notation Dist := (Distr _).
+Notation ExComp := (ExComplement _).
+
+Lemma ajBot {T : boundedLattice} (z : T) : forall a : T, a ⊔ bot = a.
+Proof.
+move=> a.
+rewrite (L2 z) -(ConnectJ z).
+by move: (TB a) => /proj2.
+Qed.
+
+Lemma amTop {T : boundedLattice} (z : T) : forall a : T, a ⊓ top = a.
+Proof.
+move=> a.
+rewrite (L2d z) -(ConnectM z).
+by move: (TB a) => /proj1.
+Qed.
+
+Definition Comp {T : boundedLattice} (a b : T ):= (a ⊔ b = top) /\ (a ⊓ b = bot).
+ 
+Lemma compUnico {T : booleanLattice} (z : T) : forall a b c : T,
+                (Comp a b /\ 
+                Comp a c) -> b = c.
+Proof.
+move=> a b c.
+rewrite /Comp. 
+move=> [[H0 H1] [H2 H3]].
+apply: antisym.
+  rewrite (ConnectM z).
+  rewrite -{2}(amTop z b).
+  rewrite -H2.
+  rewrite Dist.
+  by rewrite [b ⊓ a](L2d z) H1 (L2 z) (ajBot z) (L2d z).
+rewrite (ConnectM z).
+rewrite -{2}(amTop z (c)).
+rewrite -H0.
+rewrite Dist.
+by rewrite  [c ⊓ a](L2d z) H3 (L2 z) (ajBot z) (L2d z).
+Qed.
+
+Lemma lema4_15i {T : booleanLattice} (z : T) : (@Comp T top bot).
+Proof.
+split.
+  move: (@Top_Bottom T top) => /proj2.
+  by rewrite (ConnectJ z) (L2 z).
+move: (@Top_Bottom T bot) => /proj1.
+by rewrite (ConnectM z) (L2d z).
+Qed.
+
+Lemma lema4_15ii {T : booleanLattice} (z : T) : forall a b c : T, Comp a b -> Comp b c -> c = a.
+Proof.
+move=> a b c.
+rewrite /Comp.
+rewrite (L2 z) (L2d z).
+move=> [H0 H1] [H2 H3].
+apply: (compUnico z b).
+rewrite /Comp.
+by split.
+Qed.
+ 
+Lemma lema4_15iii {T : booleanLattice} (z : T) : forall a b caub ca cb canb : T, 
+                                         (Comp (a ⊔ b) caub -> Comp a ca -> Comp b cb -> (caub = ca ⊓ cb))
+                                         /\ (Comp (a ⊓ b) canb -> Comp a ca -> Comp b cb -> (canb = ca ⊔ cb)).
+Proof.
+move=> a b caub ca cb canb.
+move: (Distr T).
+rewrite /Distributive (Lema4_3 z) => Dis.
+split.
+  rewrite /Comp.
+  move=> [H0 H1] [H2 H3] [H4 H5].
+  apply: (compUnico z (a ⊔ b)).
+  split.
+    by [].
+  split.
+    rewrite Dis {1}[a ⊔ b](L2 z) (L1 z) H2.
+    rewrite (L1 z) H4.
+    move: (TB b) (TB a).
+    move=> /proj1/(ConnectJ z)-bTop /proj1/(ConnectJ z)-aTop.
+    by rewrite bTop aTop amTop.
+  rewrite (L2d z) Dist (L2d z) -(L1d z) H3.
+  rewrite (L1d z) [cb ⊓ b](L2d z) H5.
+  move: (TB cb) (TB ca).
+  move=> /proj2/(ConnectM z)-eBot /proj2/(ConnectM z)-dBot.
+  by rewrite (L2d z) eBot dBot ajBot.
+rewrite /Comp.
+move=> [H0 H1] [H2 H3] [H4 H5].
+apply: ((compUnico z) (a ⊓ b)).
+split.
+  by [].
+split.
+  rewrite (L2 z) Dis (L2 z) -(L1 z) H2 (L2 z).
+  rewrite (L1 z) [cb ⊔ b](L2 z) H4.
+  move: (TB cb) (TB ca).
+  move=> /proj1/(ConnectJ z)-eTop /proj1/(ConnectJ z)-dTop.
+  by rewrite eTop dTop amTop.
+rewrite Dist [a ⊓ b](L2d z) (L1d z) H3 (L2d z).
+rewrite [b ⊓ a](L2d z) (L1d z) H5 [a ⊓ bot](L2d z).
+move: (TB b) (TB a).
+move=> /proj2/(ConnectM z)-bBot /proj2/(ConnectM z)-aBot.
+by rewrite (L2d z) bBot (L2d z) aBot ajBot.
+Qed.
+ 
+Lemma lema4_15v {T : booleanLattice} (z : T) : forall a b c : T, Comp b c -> a ⊓ c = bot <-> a ≤ b.
+Proof.
+move=> a b c.
+move: (Distr T).
+rewrite /Distributive (Lema4_3 z) => DistD.
+move=> /dobl [CB [H0 H1]].
+split.
+  move=> H2.
+  rewrite (ConnectM z).
+  move: (amTop z a).
+  by rewrite -H0 Dist H2 (ajBot z) (L2d z).
+rewrite (ConnectJ z) => H.
+move: (ExComp a).
+case => a0 [aTop aBot].
+have CA : Comp a a0.
+  by [].
+move: (TB c) => /proj2.
+rewrite (ConnectM z) -{1}aBot (L2d z) (L1d z).
+move: (lema4_15iii z a b c a0 c (a ⊓ b) ) => /proj1.
+rewrite H.
+move=> /(_ CB) /(_ CA) /(_ CB)-Compl.
+by rewrite -Compl.
+Qed.
